src/Balloc.v
@@ -1817,8 +1817,13 @@ Module IAlloc.
     Definition xparams_ok xp := (BMPLen xp) <= valulen * valulen.
   End Sig.
 
-  Module Alloc := BmapAlloc Sig.
+  Module Alloc := BmapAllocCache Sig.
   Module Defs := Alloc.Defs.
+
+  Definition BmapCacheType := Alloc.BmapCacheType.
+  Definition MSLog := Alloc.MSLog.
+  Definition MSCache := Alloc.MSCache.
+  Definition mk_memstate := Alloc.mk_memstate.
 
   Definition init := Alloc.init.
 
@@ -1836,7 +1841,7 @@ Module IAlloc.
 
   Definition free_ok := Alloc.free_ok.
 
-  Definition items_per_val := Alloc.BmpSig.items_per_val.
+  Definition items_per_val := Alloc.Alloc.BmpSig.items_per_val.
 
   Hint Extern 1 ({{_}} Bind (init _ _ _) _) => apply init_ok : prog.
   Hint Extern 1 ({{_}} Bind (alloc _ _ _) _) => apply alloc_ok : prog.
@@ -1862,20 +1867,20 @@ Module IAlloc.
     apply one_lt_pow2.
   Qed.
 
-  Lemma ino_valid_goodSize : forall V FP F l m xp a prd,
-    (F * @rep V FP xp l prd)%pred m ->
+  Lemma ino_valid_goodSize : forall V FP F l m xp a prd allocc,
+    (F * @rep V FP xp l prd allocc)%pred m ->
     ino_valid xp a ->
     goodSize addrlen a.
   Proof.
     unfold rep, ino_valid.
-    unfold Alloc.rep, Alloc.Bmp.rep, Alloc.Bmp.items_valid,
-       Alloc.BmpSig.xparams_ok; intuition.
+    unfold Alloc.rep, Alloc.Alloc.rep, Alloc.Alloc.Bmp.rep, Alloc.Alloc.Bmp.items_valid,
+       Alloc.Alloc.BmpSig.xparams_ok; intuition.
     destruct_lift H.
     eapply xparams_ok_goodSize; eauto.
   Qed.
 
-  Lemma ino_valid_goodSize_pimpl : forall V FP l xp p,
-    @rep V FP xp l p <=p=> [[ forall a, ino_valid xp a -> goodSize addrlen a ]] * rep FP xp l p.
+  Lemma ino_valid_goodSize_pimpl : forall V FP l xp p allocc,
+    @rep V FP xp l p allocc <=p=> [[ forall a, ino_valid xp a -> goodSize addrlen a ]] * rep FP xp l p allocc.
   Proof.
     intros; split.
     unfold pimpl; intros.
@@ -1895,13 +1900,13 @@ Module IAlloc.
     eapply xparams_ok_goodSize; eauto.
   Qed.
 
-  Theorem ino_valid_roundtrip : forall V FP xp a F l m p,
-    (F * @rep V FP xp l p)%pred m ->
+  Theorem ino_valid_roundtrip : forall V FP xp a F l m p allocc,
+    (F * @rep V FP xp l p allocc)%pred m ->
     ino_valid xp a ->
     ino_valid xp (# (natToWord addrlen a)).
   Proof.
-    unfold rep, Alloc.rep, Alloc.Bmp.rep, Alloc.Bmp.items_valid,
-       Alloc.BmpSig.xparams_ok; intuition.
+    unfold rep, Alloc.rep, Alloc.Alloc.rep, Alloc.Alloc.Bmp.rep, Alloc.Alloc.Bmp.items_valid,
+       Alloc.Alloc.BmpSig.xparams_ok; intuition.
     destruct_lift H.
     apply ino_valid_roundtrip'; auto.
   Qed.
